KERI.lean
@@ -1,6 +1,7 @@
 import KERI.Crypto
 import KERI.CESR
 import KERI.Event
+import KERI.SAID
 import KERI.KeyState
 import KERI.KEL
 import KERI.PreRotation
